src/action.v
@@ -1,0 +1,67 @@
+From research Require Import base.
+
+Set Warnings "-notation-for-abbreviation".
+Set Asymmetric Patterns.
+
+Section WithContext.
+  Context {s : Type}.
+
+  Definition Action (t : Type) := s -> t * s.
+
+  Definition ret {t} (x : t) : Action t := fun s => (x, s).
+  Definition bind {t1 t2} (m : Action t1) (f : t1 -> Action t2) :=
+    fun r => let (x, s) := m r in (f x) s.
+
+  Definition fmap {t1 t2} (m : Action t1) (f : t1 -> t2) :=
+    bind m (fun x => ret (f x)).
+
+  Definition pass : Action unit := ret tt.
+
+  Definition get : Action s := fun s => (s, s).
+  Definition put (x : s) : Action unit := fun _ => (tt, x).
+  Definition modify (f : s -> s) : Action unit := fun s => (tt, f s).
+
+  Definition runAction  {a} (m : Action a) (x : s) := m x.
+  Definition runAction1 {a} (m : Action a) := (fst ∘ (runAction (a := a) m)).
+  Definition runAction2 {a} (m : Action a) := (snd ∘ (runAction (a := a) m)).
+End WithContext.
+
+Notation ActionUnit := (Action unit).
+
+Declare Scope action_scope.
+Delimit Scope action_scope with action.
+
+Infix ">>=" := bind (at level 60) : action_scope.
+Infix ">>|" := fmap (at level 60) : action_scope.
+
+Notation "'{{' e '}}'" := (e%action : Action _).
+
+Notation "'let%bind' x ':=' e1 'in' e2" :=
+  (e1 >>= (fun x => e2))%action
+    (at level 100, x pattern, e2 at level 200, right associativity) : action_scope.
+
+Notation "'let%map' x ':=' e1 'in' e2" :=
+  (e1 >>| (fun x => e2))%action
+    (at level 100, x pattern, e2 at level 200, right associativity) : action_scope.
+
+Notation "'let%read' x ':=' e1 'in' e2" :=
+  (get >>| e1 >>= (fun x => e2))%action
+    (at level 100, x at next level, e2 at level 200, right associativity) : action_scope.
+
+Notation "'let%write' x ':=' e1 'in' e2" :=
+  (modify (set x (fun _ => e1)) >>= (fun _ => e2))%action
+    (at level 100, x at next level, e2 at level 200, right associativity) : action_scope.
+
+Notation "'let%modify' x ':=' e1 'in' e2" :=
+  (modify (set x e1) >>= (fun _ => e2))%action
+    (at level 100, x at next level, e2 at level 200, right associativity) : action_scope.
+
+Notation "'let%call' x ':=' e1 'on' field 'in' e2" :=
+  (get >>= (fun s =>
+              let (x, s') := runAction e1 (field s) in
+              put (set field (fun _ : _ => s') s) >>= (fun _ => e2)))%action
+    (at level 100, x pattern, e1 at next level, field at next level,
+      e2 at level 200, right associativity) : action_scope.
+
+Notation " 'when' c 'then' e " := (if c then e else pass) (at level 200) : action_scope.
+Notation " 'guard' c 'then' e " := (if c then e else pass) (at level 200) : action_scope.
