src/add_multiply.v
@@ -1,0 +1,214 @@
+From research Require Import base bit circuit multiplier fifo regfile.
+From stdpp Require Import fin finite.
+
+Notation Maybe := @option.
+
+Inductive Instr :=
+| Add (rd rs1 rs2 : Bit 5)
+| Addi (rd rs1 : Bit 5) (imm : Bit 4)
+| Mul (rd rs1 rs2 : Bit 5)
+| Unknown.
+
+Inductive method :=
+| GetIReq
+| GetIResp (resp : Instr)
+| Rule.
+
+Inductive state :=
+| State__Fetch
+| State__Decode
+| State__Execute.
+
+Inductive implLeakage := .
+
+Instance state__EqDecision : EqDecision state.
+Proof.
+  solve_decision.
+Defined.
+
+Module AddMultiply.
+  Inductive D2E :=
+  | DAdd (rd : Bit 5) (v1 v2 : Bit 4)
+  | DMul (rd : Bit 5) (v1 v2 : Bit 4).
+
+  Record t :=
+    { m : Multiplier.t
+    ; rf : RegFile.t 4 5
+    ; pc : Bit 32
+    ; fromImem : Fifo.t Instr
+    ; toImem : Fifo.t (Bit 32)
+    ; d2e : Fifo.t D2E
+    ; st : state
+    ; trace : list implLeakage
+    }.
+
+  Definition mk :=
+    {| m := Multiplier.mk
+    ; rf := RegFile.mk
+    ; pc := 0%bv
+    ; fromImem := Fifo.mk
+    ; toImem := Fifo.mk
+    ; d2e := Fifo.mk
+    ; st := State__Fetch
+    ; trace := []
+    |}.
+
+  Definition getIReq :=
+    {{ let%read toImem0 := toImem in
+       if (Fifo.notEmpty toImem0) then
+         let%call d := Fifo.deq on toImem in
+         match d with
+         | Valid d => ret d
+         | Invalid => ret 0%bv
+         end
+       else
+         ret 0%bv
+    }}.
+
+  Definition getIResp instr :=
+    {{ let%read fromImem0 := fromImem in
+       guard (Fifo.notFull fromImem0) then
+         let%call _ := Fifo.enq instr on fromImem in
+         pass
+    }}.
+
+  Definition fetch :=
+    {{ let%read pc0 := pc in
+       let%read toImem0 := toImem in
+       guard (Fifo.notFull toImem0) then
+         let%call _ := Fifo.enq pc0 on toImem in
+         let%write st := State__Decode in
+         pass
+    }}.
+
+  Definition decode :=
+    {{ let%read fromImem0 := fromImem in
+       let%read toImem0   := toImem in
+       let%read d2e0      := d2e in
+       let%read rf0       := rf in
+       guard (Fifo.notFull d2e0 && Fifo.notEmpty fromImem0 && Fifo.notFull toImem0) then
+         let%call instr := Fifo.deq on fromImem in
+         match instr with
+         | Valid Unknown =>
+             let%write st := State__Fetch in pass
+         | Valid (Add rd rs1 rs2) =>
+             let v1 := RegFile.sub rs1 rf0 in
+             let v2 := RegFile.sub rs2 rf0 in
+             let%call _ := Fifo.enq (DAdd rd v1 v2) on d2e in
+             let%write st := State__Execute in
+             pass
+         | Valid (Mul rd rs1 rs2) =>
+             let v1 := RegFile.sub rs1 rf0 in
+             let v2 := RegFile.sub rs2 rf0 in
+             let%call _ := Fifo.enq (DMul rd v1 v2) on d2e in
+             let%write st := State__Execute in
+             pass
+         | Valid (Addi rd rs1 imm) =>
+             let v1 := RegFile.sub rs1 rf0 in
+             let%call _ := Fifo.enq (DAdd rd v1 imm) on d2e in
+             let%write st := State__Execute in
+             pass
+         | Invalid => pass
+         end
+    }}.
+
+  Definition executeAdd rd v1 v2 :=
+    {{ let%call _ := Fifo.deq on d2e in
+       let%call _ := RegFile.upd rd (v1 + v2)%bv on rf in
+       let%write st := State__Fetch in
+       let%modify pc := fun pc => (pc `+Z` 4)%bv in
+       pass
+    }}.
+
+  Definition executeMul rd v1 v2 :=
+    {{ let%read m0 := m in
+       match Multiplier.st m0 with
+       | State__Empty =>
+           let%call _ := Multiplier.enq v1 v2 on m in
+           pass
+       | State__Busy =>
+           let%call _ := Multiplier.rule on m in
+           pass
+       | State__Full =>
+           let%call v := Multiplier.deq on m in
+           match v with
+           | Valid v =>
+               let%call _ := Fifo.deq on d2e in
+               let%call _ := RegFile.upd rd (truncate v) on rf in
+               let%write st := State__Fetch in
+               let%modify pc := fun pc => (pc `+Z` 4)%bv in
+               pass
+           | Invalid => pass
+           end
+       end
+    }}.
+
+  Definition execute :=
+    {{ let%read d2e0 := d2e in
+       guard (Fifo.notEmpty d2e0) then
+         let instr := Fifo.first d2e0 in
+         match instr with
+         | Valid (DAdd rd v1 v2) => executeAdd rd v1 v2
+         | Valid (DMul rd v1 v2) => executeMul rd v1 v2
+         | Invalid => pass
+         end
+    }}.
+
+  Definition rule :=
+    {{ let%read st0 := st in
+       match st0 with
+       | State__Fetch => fetch
+       | State__Decode => decode
+       | State__Execute => execute
+       end
+    }}.
+
+  Instance circuit : Circuit :=
+    {| circuitInit := mk
+    ; circuitResult m :=
+        match m with
+        | GetIReq => Bit 32
+        | GetIResp _ => unit
+        | Rule => unit
+        end
+    ; circuitCall m :=
+        match m with
+        | GetIReq => getIReq
+        | GetIResp resp => getIResp resp
+        | Rule => rule
+        end
+    ; circuitTrace := trace
+    |}.
+End AddMultiply.
+
+Section example.
+  Notation runCircuit := (runCircuit (c := AddMultiply.circuit)).
+
+  Definition ms :=
+    [Rule
+     ; GetIReq
+     ; GetIResp (Addi 1%bv 0%bv 3%bv)
+     ; Rule
+     ; Rule
+     ; Rule
+     ; Rule
+     ; Rule
+     ; GetIResp (Addi 2%bv 0%bv 4%bv)
+     ; GetIReq
+     ; Rule
+     ; Rule
+     ; Rule
+     ; GetIReq
+     ; GetIResp (Mul 3%bv 1%bv 2%bv)
+     ; Rule
+     ; Rule
+     ; Rule
+     ; Rule
+     ; Rule
+     ; Rule
+     ; Rule
+     ; Rule
+    ].
+
+  Eval vm_compute in runCircuit ms.
+End example.
