src/bit.v
@@ -17,22 +17,5 @@ Definition zeroExtend {n z} := bv_zero_extend (n := n) z.
 Definition truncate {n z} := bv_zero_extend (n := n) z.
 Definition signExtend {n z} := bv_sign_extend (n := n) z.
 Definition concat {n n1 n2} := bv_concat n (n1 := n1) (n2 := n2).
-Definition select {n1 n2} (h l : N) (b : Bit n1) : Bit n2 :=
-  zeroExtend (Z_to_bv (h - l + 1) (b.(bv_unsigned) ≫ Z.of_N l)) : Bit n2.
 
 Infix "++:" := concat (at level 60, right associativity) : bv_scope.
-Notation "b [[ h ; l ]]" := (select h l b) : bv_scope.
-
-Lemma bit_1_not_zero_then_one : forall (x : Bit 1), x <> 0 <-> x = 1.
-Proof.
-  induction x using bv_1_ind; equality.
-Qed.
-
-Lemma decide_bit1 (x : Bit 1) : {x = 0} + {x = 1}.
-Proof.
-  refine (
-      if decide (x = 0) then _ else _
-  ).
-  - abstract (left; exact e).
-  - abstract (right; apply bit_1_not_zero_then_one; exact n).
-Qed.
