src/fifo.v
@@ -1,0 +1,36 @@
+From research Require Import base circuit.
+
+Module Fifo.
+  Section WithContext.
+    Context (a : Type).
+
+    Record t := { first : Maybe a }.
+
+    Definition mk := {| first := Invalid |}.
+
+    Definition notEmpty s := bool_decide (s.(first) <> Invalid).
+    Definition notFull s := bool_decide (s.(first) = Invalid).
+
+    Definition enq in__a :=
+      {{ let%read first0 := first in
+         guard decide (first0 = Invalid) then
+           let%write first := Valid in__a in
+           pass
+      }}.
+
+    Definition deq :=
+      {{ let%read first0 := first in
+         if decide (first0 <> Invalid) then
+           let%write first := Invalid in
+           ret first0
+         else
+           ret Invalid
+      }}.
+  End WithContext.
+
+  Arguments mk {_}.
+  Arguments enq {_} (_ _).
+  Arguments deq {_} (_).
+  Arguments notEmpty {_} (_).
+  Arguments notFull {_} (_).
+End Fifo.
