src/regfile.v
@@ -1,0 +1,27 @@
+From research Require Import base bit circuit.
+From stdpp Require Import fin finite vector.
+
+Module RegFile.
+  Section WithContext.
+    Context (b : N) (sz : N) {H0 : BvWf b 0} {H1 : BvWf sz 0}.
+
+    Record t := { contents : Vector (Bit b) (card (Bit sz)) }.
+
+    Definition mk := {| contents := mkVector 0%bv (card (Bit sz)) |}.
+
+    Definition sub (addr : Bit sz) (t : t) :=
+      if decide (addr = 0)%bv then
+        0%bv
+      else
+        t.(contents) !!! encode_fin addr.
+
+    Definition upd (addr : Bit sz) (data : Bit b) :=
+      {{ let%modify contents := vinsert (encode_fin addr) data in
+         pass
+      }}.
+  End WithContext.
+
+  Arguments mk {_ _ _}.
+  Arguments sub {_ _ _ _}.
+  Arguments upd {_ _}.
+End RegFile.
